PiLL/Semantics/EnvStep/Basic.lean
@@ -1,0 +1,64 @@
+import PiLL.Model.HyperEnvironment.Basic
+import PiLL.Model.STypes.Notation
+import PiLL.Semantics.Labels
+
+inductive EnvStepₘ : HyperEnv → Lbl → HyperEnv → Prop where
+  | one
+      {x : FPName} :
+      EnvStepₘ [[x ∶ 1]] (x⟦⟧) ∅
+  | tensor
+      {Γ Δ : Env} {x x' : FPName} {A B : Types}
+      (hF : x' ∉ HyperEnv.names [x ∶ A ⨂ B :: Γ‚ Δ]) :
+      EnvStepₘ [x ∶ A ⨂ B :: Γ‚ Δ] (x⟦x'⟧) ([x' ∶ A :: Γ] |ₕ [x ∶ B :: Δ])
+  | bot
+      {Γ : Env} {x : FPName} :
+      EnvStepₘ [x ∶ ⊥ :: Γ] (x⸨⸩) [Γ]
+  | parr
+      {Γ : Env} {x x' : FPName} {A B : Types}
+      (hF : x' ∉ HyperEnv.names [x ∶ A ⅋ B :: Γ]) :
+      EnvStepₘ [x ∶ A ⅋ B :: Γ] (x⸨x'⸩) [x' ∶ A :: x ∶ B :: Γ]
+  | par₁
+      {𝒢 𝒢' ℋ : HyperEnv} {l : Lbl} :
+      EnvStepₘ 𝒢 l 𝒢' →
+      -----------------------------
+      EnvStepₘ (𝒢 |ₕ ℋ) l (𝒢' |ₕ ℋ)
+  | par₂
+      {𝒢 ℋ ℋ': HyperEnv} {l : Lbl} :
+      EnvStepₘ ℋ l ℋ' →
+      -----------------------------
+      EnvStepₘ (𝒢 |ₕ ℋ) l (𝒢 |ₕ ℋ')
+  | syn
+      {𝒢 𝒢' ℋ ℋ': HyperEnv} {l l' : Act} :
+      EnvStepₘ 𝒢 l 𝒢' → EnvStepₘ ℋ l' ℋ' →
+      --------------------------------------------------
+      EnvStepₘ (𝒢 |ₕ ℋ) (l |ₗ l') (𝒢' |ₕ ℋ')
+  | one_bot
+      {𝒢 : HyperEnv} {Γ : Env} {x y : FPName} :
+      EnvStepₘ (𝒢 |ₕ [[x ∶ 1]] |ₕ [y ∶ ⊥ :: Γ]) (x⟦⟧ |ₗ y⸨⸩) (𝒢 |ₕ [Γ]) →
+      ---------------------------------------------------------------
+      EnvStepₘ (𝒢 |ₕ [Γ]) (τ) (𝒢 |ₕ [Γ])
+  | tensor_parr
+      {𝒢 : HyperEnv} {Γ Δ Ξ : Env} {x x' y y': FPName} {A B : Types} :
+      EnvStepₘ
+        (𝒢 |ₕ [x ∶ A ⨂ B :: Γ‚ Δ] |ₕ [y ∶ Aᗮ ⅋ Bᗮ :: Ξ])
+        (x⟦x'⟧ |ₗ y⸨y'⸩)
+        (𝒢 |ₕ [x ∶ B :: Δ] |ₕ [x' ∶ A :: Γ] |ₕ [y' ∶ Aᗮ :: y ∶ Bᗮ :: Ξ]) →
+      ------------------------------------------------------------------
+      EnvStepₘ (𝒢 |ₕ [Γ‚ Δ‚ Ξ]) (τ) (𝒢 |ₕ [Γ‚ Δ‚ Ξ])
+  | res
+      {𝒢 𝒢' : HyperEnv} {Γ Γ' Δ Δ' : Env} {x y : FPName} {A : Types} {l : Lbl}
+      (hFx : x ∉ l.i ∪ l.f) (hFy : y ∉ l.i ∪ l.f) :
+      EnvStepₘ (𝒢 |ₕ [x ∶ A :: Γ] |ₕ [y ∶ Aᗮ :: Δ]) (l) (𝒢' |ₕ [x ∶ A :: Γ'] |ₕ [y ∶ Aᗮ :: Δ']) →
+      -------------------------------------------------------------------------------------
+      EnvStepₘ (𝒢 |ₕ [Γ‚ Δ]) l (𝒢' |ₕ [Γ'‚ Δ'])
+  ------- Additional Structural / Exchange Rules -------
+  | perm_env {𝒢 ℋ : HyperEnv} {Γ Γ' : Env} {l : Lbl} (hP1 : Γ ~ Γ') :
+      (hES : EnvStepₘ (Γ :: 𝒢) l ℋ) →
+      ---------------------------------
+      EnvStepₘ (Γ' :: 𝒢) l ℋ
+  | perm_hyper {𝒢 𝒢' ℋ ℋ' : HyperEnv} {l : Lbl} (hP1 : 𝒢 ~ 𝒢') (hP2 : ℋ ~ ℋ') :
+      (hES : EnvStepₘ 𝒢 l ℋ) →
+      -------------------------
+      EnvStepₘ 𝒢' l ℋ'
+
+instance : HasStep HyperEnv Lbl HyperEnv where step := EnvStepₘ
