PiLL/Semantics/JudgementStep/Inversion/Res.lean
@@ -1,0 +1,120 @@
+import PiLL.Semantics.JudgementStep.Basic
+import PiLL.Model.HyperEnvironment.Lemmas.Basic
+
+
+
+
+
+
+
+
+
+
+
+
+
+
+
+
+
+-- FIXME: Move to hyperenvironments
+lemma HyperEnv.Perm.length_eq {𝒢 ℋ : HyperEnv} (hP : 𝒢 ~ ℋ) :
+  𝒢.length = ℋ.length := by
+  induction hP with
+  | nil => rfl
+  | cons _ _ ih => simp [ih]
+  | swap => simp
+  | trans _ _ ih1 ih2 => exact ih1.trans ih2
+
+
+
+
+lemma TypingStepₘ_preserves_disjoint_or_merges {n n' : Nat} {P P' : Proc}
+  {ℋ ℋ' : HyperEnv} {l : Lbl} {𝒟' : n' ⊢ P' ∷ ℋ'}
+  (𝒟 : n ⊢ P ∷ ℋ) (hStep : TypingStepₘ 𝒟 l 𝒟')
+
+  {𝒢 : HyperEnv} {Γ Δ : Env} {A : Types} {x y : FPName}
+  (hxl : x ∉ l.f ∪ l.i) (hyl : y ∉ l.f ∪ l.i)
+  (hP : ℋ ~ 𝒢 |ₕ [x ∶ A :: Γ] |ₕ [y ∶ Aᗮ :: Δ]) :
+  (∃ 𝒢' Γ' Δ', ℋ ~ 𝒢' |ₕ [x ∶ A :: Γ'] |ₕ [y ∶ Aᗮ :: Δ']) ∨
+  (∃ 𝒢' ΓΔ', ℋ ~ 𝒢' |ₕ [x ∶ A :: ΓΔ' ++ [y ∶ Aᗮ]]) := by
+  induction hStep generalizing 𝒢 Γ Δ
+
+  case one | bot | tensor | parr =>
+    exfalso
+    have h_len := HyperEnv.Perm.length_eq hP
+    simp only [List.length_singleton, List.length_append] at h_len
+    omega
+
+  case par₁ =>
+
+
+
+
+    sorry
+  case par₂ => sorry
+
+
+
+  case syn => sorry
+  case one_bot => sorry
+  case tensor_parr => sorry
+  case res => sorry
+  case perm_env =>
+
+
+
+
+    sorry
+  case perm_hyper =>
+
+
+
+    sorry
+
+
+
+
+
+
+
+
+
+
+
+
+
+
+
+
+
+-- TODO: Move ProcStep, EnvStep, and Typing and HyperEnv lemmas to respective files
+-- TODO: Prove Session fidelity, erasure, type preservation, Session fidelity for πLL
+-- TODO: Delete Single files in favor of the new folder structure
+
+
+-- FIXME: Typing_preserves_proc_congr
+-- FIXME: Proof showing substitution avoids capture
+-- FIXME: Proof showing AlphaEq is equivalent to = between Procs
+
+-- FIXME: Prove name substitution only being applied to free names?
+--        (Basically just Typing_f_eq_names since 𝒢.names = P.f => Typing.substNames is
+--         being applied to P.f)
+
+
+-- NOTE: shows the proof lean found using the simp_all tactic show_term { simp_all }
+-- NOTE: Remember that lemmas exist for duplicating a process and disposing
+
+-- TODO: Find different syntax for open?
+-- TODO: Use NameSpaces instead of having e.g. HyperEnv._____ everywhere
+/- TODO:
+  Refine / organize the various "Lemmas" folders to be more organized instead of
+  simply throwing every lemma into one file
+-/
+-- TODO: Change lemma naminig and dot notation interactions to follow standard pattern
+-- TODO: Change HyperEnv.Nodup def to match Env
+-- TODO: Edit files to follow the new linters lean has added
+/- TODO:
+  - Maybe remove all_fresh from one_bot signature and make it like tensor_parr and
+  do inline induction instead.
+-/
