PiLL/Semantics/JudgementStep/Inversion/Tensor_Parr.lean
@@ -1,0 +1,339 @@
+import PiLL.Semantics.JudgementStep.Basic
+import PiLL.Semantics.JudgementStep.Inversion.Tensor
+import PiLL.Semantics.JudgementStep.Inversion.Parr
+import PiLL.Model.HyperEnvironment.Lemmas.Basic
+import PiLL.Model.HyperEnvironment.Lemmas.Extraction.Tensor_Parr_res
+import PiLL.Model.HyperEnvironment.Lemmas.Extraction.Tensor_Parr_Res_Crosslinked
+
+lemma TypingStepₘ_inv_tensor_parr_existential {n n' : Nat} {P P' : Proc} {𝒢 𝒢' : HyperEnv}
+  {x x' y y' : FPName} {𝒟 : n ⊢ P ∷ 𝒢} {𝒟' : n' ⊢ P' ∷ 𝒢'}
+  (hStep : TypingStepₘ 𝒟 (x⟦x'⟧ |ₗ y⸨y'⸩) 𝒟') :
+  (∃ 𝒢ᵣ Γᵣ Δᵣ Ξᵣ A B C D,
+    (𝒢 ~ 𝒢ᵣ |ₕ [x ∶ A ⨂ B :: Γᵣ‚ Δᵣ] |ₕ [y ∶ C ⅋ D :: Ξᵣ]) ∧
+    (𝒢' ~ 𝒢ᵣ |ₕ [x ∶ B :: Δᵣ] |ₕ [x' ∶ A :: Γᵣ] |ₕ [y' ∶ C :: y ∶ D :: Ξᵣ])) ∨
+  (∃ 𝒢ᵣ Γᵣ Δᵣ Ξᵣ A B C D,
+    (𝒢 ~ 𝒢ᵣ |ₕ [x ∶ A ⨂ B :: Γᵣ‚ Δᵣ ++ y ∶ C ⅋ D :: Ξᵣ]) ∧
+    ((𝒢' ~ 𝒢ᵣ |ₕ [x ∶ B :: Δᵣ] |ₕ [x' ∶ A :: Γᵣ ++ y' ∶ C :: y ∶ D :: Ξᵣ]) ∨
+     (𝒢' ~ 𝒢ᵣ |ₕ [x' ∶ A :: Γᵣ] |ₕ [x ∶ B :: Δᵣ ++ y' ∶ C :: y ∶ D :: Ξᵣ]))) := by
+  generalize hl : (x⟦x'⟧ |ₗ y⸨y'⸩) = l at hStep
+  induction hStep <;> try simp only [HasBracket.brack, HasParen.paren, reduceCtorEq,
+    Lbl.par.injEq] at hl
+  case par₁ ih =>
+    expose_names
+    subst hl
+    simp only [HasBracket.brack, HasParen.paren, true_implies] at ih
+    rcases ih with ⟨𝒢ₙ, Γₙ, Δₙ, Ξₙ, A, B, C, D, hP, hP'⟩ | ⟨𝒢ₙ, Γₙ, Δₙ, Ξₙ, A, B, C, D, hP, hP'⟩
+    · left
+      refine ⟨𝒢ₙ |ₕ ℋ, Γₙ, Δₙ, Ξₙ, A, B, C, D,  ?_, ?_⟩
+      · apply HyperEnv.Perm_rotate_rhs_left
+        rw [← HyperEnv.merge_assoc]
+        apply HyperEnv.Perm_merge_cancel_right_inv
+        exact HyperEnv.Perm_rotate_rhs_right hP
+      · rw [HyperEnv.merge_assoc, HyperEnv.merge_assoc]
+        apply HyperEnv.Perm_rotate_rhs_right
+        apply HyperEnv.Perm_merge_cancel_right_inv
+        apply HyperEnv.Perm_rotate_rhs_right
+        rw [← HyperEnv.merge_assoc]
+        exact hP'
+    · right
+      refine ⟨𝒢ₙ |ₕ ℋ, Γₙ, Δₙ, Ξₙ, A, B, C, D,  ?_, ?_⟩
+      · have h1 : 𝒢_1 |ₕ ℋ ~ (𝒢ₙ |ₕ [x ∶ A ⨂ B :: Γₙ‚ Δₙ ++ y ∶ C ⅋ D :: Ξₙ]) |ₕ ℋ :=
+          HyperEnv.Perm.merge hP (by rfl)
+        have h2 : (𝒢ₙ |ₕ [x ∶ A ⨂ B :: Γₙ‚ Δₙ ++ y ∶ C ⅋ D :: Ξₙ]) |ₕ ℋ ~
+          (𝒢ₙ |ₕ ℋ) |ₕ [x ∶ A ⨂ B :: Γₙ‚ Δₙ ++ y ∶ C ⅋ D :: Ξₙ] := by
+          apply HyperEnv.Perm_rotate_rhs_right
+          apply HyperEnv.Perm_merge_cancel_right_inv
+          exact HyperEnv.Perm.merge_comm
+        exact h1.trans h2
+      · rcases hP' with hP'1 | hP'2
+        · left
+          rw [HyperEnv.merge_assoc]
+          apply HyperEnv.Perm_rotate_rhs_right
+          apply HyperEnv.Perm_merge_cancel_right_inv
+          apply HyperEnv.Perm_rotate_rhs_right
+          exact hP'1
+        · right
+          rw [HyperEnv.merge_assoc]
+          apply HyperEnv.Perm_rotate_rhs_right
+          apply HyperEnv.Perm_merge_cancel_right_inv
+          apply HyperEnv.Perm_rotate_rhs_right
+          exact hP'2
+  case par₂ ih =>
+    expose_names
+    subst hl
+    simp only [HasBracket.brack, HasParen.paren, true_implies] at ih
+    rcases ih with ⟨𝒢ₙ, Γₙ, Δₙ, Ξₙ, A, B, C, D, hP, hP'⟩ | ⟨𝒢ₙ, Γₙ, Δₙ, Ξₙ, A, B, C, D, hP, hP'⟩
+    · left
+      refine ⟨𝒢_1 |ₕ 𝒢ₙ , Γₙ, Δₙ, Ξₙ, A, B, C, D,  ?_, ?_⟩
+      · simp only [HyperEnv.merge_assoc]
+        apply HyperEnv.Perm_merge_cancel_left_inv
+        rw [← HyperEnv.merge_assoc]
+        exact hP
+      · simp only [HyperEnv.merge_assoc]
+        apply HyperEnv.Perm_merge_cancel_left_inv
+        simp only [← HyperEnv.merge_assoc]
+        exact hP'
+    · right
+      refine ⟨𝒢_1 |ₕ 𝒢ₙ , Γₙ, Δₙ, Ξₙ, A, B, C, D,  ?_, ?_⟩
+      · simp only [HyperEnv.merge_assoc]
+        apply HyperEnv.Perm_merge_cancel_left_inv
+        exact hP
+      · rcases hP' with hP'1 | hP'2
+        · left
+          simp only [HyperEnv.merge_assoc]
+          apply HyperEnv.Perm_merge_cancel_left_inv
+          simp only [← HyperEnv.merge_assoc]
+          exact hP'1
+        · right
+          simp only [HyperEnv.merge_assoc]
+          apply HyperEnv.Perm_merge_cancel_left_inv
+          simp only [← HyperEnv.merge_assoc]
+          exact hP'2
+  case syn ih1 ih2 =>
+    expose_names
+    obtain ⟨hl1, hl2⟩ := hl
+    subst hl1 hl2
+    obtain ⟨𝒢ᵣ, Γ₁, Γ₂, A, B, hxx', hP_pre, hP_post⟩ := TypingStepₘ_inv_tensor_existential h₁
+    obtain ⟨𝒢ᵣ', Δ, C, D, hyy', hP_pre', hP_post'⟩ := TypingStepₘ_inv_parr_existential h₂
+    left
+    refine ⟨(𝒢ᵣ |ₕ 𝒢ᵣ'), Γ₁, Γ₂, Δ, A, B, C, D, ?_, ?_⟩
+    · have hP_merge := HyperEnv.Perm.merge hP_pre hP_pre'
+      have hP_trans : 𝒢ᵣ |ₕ [x ∶ A ⨂ B :: Γ₁‚ Γ₂] |ₕ (𝒢ᵣ' |ₕ [y ∶ C ⅋ D :: Δ]) ~
+        𝒢ᵣ |ₕ 𝒢ᵣ' |ₕ [x ∶ A ⨂ B :: Γ₁‚ Γ₂] |ₕ [y ∶ C ⅋ D :: Δ] := by
+        simp only [HyperEnv.merge_assoc]
+        apply HyperEnv.Perm_merge_cancel_left_inv
+        simp only [← HyperEnv.merge_assoc]
+        apply HyperEnv.Perm_rotate_rhs_left
+        simp only [HyperEnv.merge_assoc]
+        exact HyperEnv.Perm_merge_cancel_left_inv HyperEnv.Perm.merge_comm
+      exact hP_merge.trans hP_trans
+    · have hP_merge' := HyperEnv.Perm.merge hP_post hP_post'
+      have hP_trans' : 𝒢ᵣ |ₕ [x ∶ B :: Γ₂] |ₕ [x' ∶ A :: Γ₁] |ₕ (𝒢ᵣ' |ₕ [y' ∶ C :: y ∶ D :: Δ]) ~
+        𝒢ᵣ |ₕ 𝒢ᵣ' |ₕ [x ∶ B :: Γ₂] |ₕ [x' ∶ A :: Γ₁] |ₕ [y' ∶ C :: y ∶ D :: Δ] := by
+        simp only [HyperEnv.merge_assoc]
+        apply HyperEnv.Perm_merge_cancel_left_inv
+        conv_rhs => rw [← HyperEnv.merge_assoc]
+        apply HyperEnv.Perm_rotate_rhs_left
+        rw [HyperEnv.merge_assoc]
+        apply HyperEnv.Perm_merge_cancel_left_inv
+        rw [HyperEnv.merge_assoc]
+        apply HyperEnv.Perm_merge_cancel_left_inv
+        exact HyperEnv.Perm.merge_comm
+      exact  hP_merge'.trans hP_trans'
+  case res ih =>
+    expose_names
+    subst hl
+    simp only [Lbl.f, fNamesAct, Finset.singleton_union, Lbl.i, iNamesAct, Finset.union_insert,
+      Finset.insert_union, Finset.mem_insert, Finset.mem_singleton, not_or, ← ne_eq] at hlx hly
+    simp only [Finset.union_assoc, Finset.mem_union, not_or] at hx_pre hy_pre hx_post hy_post
+    rcases ih rfl with ⟨𝒢ᵣ, Γᵣ, Δᵣ, Ξᵣ, A, B, C, D, hP_pre, hP_post⟩ |
+      ⟨𝒢ᵣ, Γᵣ, Δᵣ, Ξᵣ, A, B, C, D, hP_pre, hP_post_or⟩
+    · rcases HyperEnv.Perm.extract_tensor_parr_res
+          hP_pre hP_post
+          hlx.2.1 hlx.1 hlx.2.2.1 hlx.2.2.2
+          hly.2.1 hly.1 hly.2.2.1 hly.2.2.2
+          hneq
+          hx_pre.2.1 hy_pre.2.1 hx_post.2.1 hy_post.2.1
+          hx_pre.2.2.2 hy_pre.2.2.1
+      with ⟨𝒢ₙ, Γₙ, Δₙ, Ξₙ, h_pre_res, h_post_res⟩ | ⟨𝒢ₙ, Γₙ, Δₙ, Ξₙ, h_pre_res, h_post_res⟩
+      · left
+        refine ⟨𝒢ₙ, Γₙ, Δₙ, Ξₙ, A, B, C, D, h_pre_res, h_post_res⟩
+      · right
+        refine ⟨𝒢ₙ, Γₙ, Δₙ, Ξₙ, A, B, C, D, h_pre_res, h_post_res⟩
+    · right
+      obtain ⟨𝒢ₙ, Γₙ, Δₙ, Ξₙ, h_pre_res, h_post_res⟩ :=
+        HyperEnv.Perm.extract_tensor_parr_res_crosslinked
+          hP_pre hP_post_or hlx.1 hlx.2.2.2 hly.1 hly.2.2.2 hlx.2.1
+          hly.2.1 hly.2.2.1 hlx.2.2.1 hneq hx_pre.2.1 hx_post.2.1
+          hy_pre.2.1 hy_post.2.1 hx_pre.2.2.1 hx_post.2.2.1 hx_pre.2.2.2
+          hx_post.2.2.2 hy_pre.2.2.1 hy_post.2.2.1 hy_pre.2.2.2 hy_post.2.2.2
+      refine ⟨𝒢ₙ, Γₙ, Δₙ, Ξₙ, A, B, C, D, ?_, ?_⟩
+      · exact h_pre_res
+      · exact h_post_res
+  case perm_env ih =>
+    expose_names
+    subst hl
+    simp only [HasBracket.brack, HasParen.paren, true_implies] at ih
+    rcases ih with ⟨𝒢ₙ, Γₙ, Δₙ, Ξₙ, A, B, C, D, hP, hP'⟩ | ⟨𝒢ₙ, Γₙ, Δₙ, Ξₙ, A, B, C, D, hP, hP'_or⟩
+    · left
+      refine ⟨𝒢ₙ, Γₙ, Δₙ, Ξₙ, A, B, C, D, ?_, hP'⟩
+      exact (HyperEnv.Perm.cons (ℋ := 𝒢_1) hP1.symm (by rfl)).trans hP
+    · right
+      refine ⟨𝒢ₙ, Γₙ, Δₙ, Ξₙ, A, B, C, D, ?_, hP'_or⟩
+      exact (HyperEnv.Perm.cons (ℋ := 𝒢_1) hP1.symm (by rfl)).trans hP
+  case perm_hyper ih =>
+    expose_names
+    subst hl
+    simp only [HasBracket.brack, HasParen.paren, true_implies] at ih
+    rcases ih with ⟨𝒢ₙ, Γₙ, Δₙ, Ξₙ, A, B, C, D, hP, hP'⟩ | ⟨𝒢ₙ, Γₙ, Δₙ, Ξₙ, A, B, C, D, hP, hP'_or⟩
+    · left
+      refine ⟨𝒢ₙ, Γₙ, Δₙ, Ξₙ, A, B, C, D, ?_, ?_⟩
+      · exact hP1.symm.trans hP
+      · exact hP2.symm.trans hP'
+    · right
+      refine ⟨𝒢ₙ, Γₙ, Δₙ, Ξₙ, A, B, C, D, ?_, ?_⟩
+      · exact hP1.symm.trans hP
+      · rcases hP'_or with hP'_L | hP'_R
+        · left ; exact hP2.symm.trans hP'_L
+        · right ; exact hP2.symm.trans hP'_R
+
+lemma TypingStepₘ_inv_tensor_parr_source {n n' : Nat} {P P' : Proc} {𝒢 𝒢' : HyperEnv}
+  {x x' y y' : FPName} {A B : Types} {Γ Δ : Env} {𝒟' : n' ⊢ P' ∷ 𝒢'}
+  (𝒟 : n ⊢ P ∷ 𝒢 |ₕ [x ∶ A :: Γ] |ₕ [y ∶ B :: Δ])
+  (hStep : TypingStepₘ 𝒟 (x⟦x'⟧ |ₗ y⸨y'⸩) 𝒟') :
+  ∃ (C D E F : Types) (Γ₁ Γ₂ : Env),
+    A = C ⨂ D ∧
+    B = E ⅋ F ∧
+    Γ ~ Γ₁‚ Γ₂ ∧
+    𝒢' ~ 𝒢 |ₕ [x ∶ D :: Γ₂] |ₕ [x' ∶ C :: Γ₁] |ₕ [y' ∶ E :: y ∶ F :: Δ] := by
+  obtain h_left | h_right := TypingStepₘ_inv_tensor_parr_existential hStep
+  · obtain ⟨𝒢ᵣ, Γᵣ, Δᵣ, Ξᵣ, C, D, E, F, hP_pre, hP_post⟩ := h_left
+    have ⟨hdn, hpw⟩ := Typing_preserves_linearity 𝒟
+    have ⟨⟨hx𝒢, hxΓ, hxΔ⟩, ⟨hy𝒢, hyΓ, hyΔ⟩⟩ := Typing_res_fresh 𝒟
+    simp only [List.append_assoc, List.cons_append, List.nil_append,
+      HyperEnv.PairwiseDisjoint_merge, List.mem_cons, List.not_mem_nil, or_false,
+      Env.names_distributes, Finset.singleton_union, Finset.disjoint_insert_right,
+      Env.mem_pair_fst_in_names_iff, not_exists, forall_eq, forall_eq_or_imp] at hpw
+    have hDΓΔ := HyperEnv.PairwiseDisjoint_implies_disjoint hpw.2.1
+    have hxLHS : ∃ Γ', Γ' ∈ 𝒢 |ₕ [x ∶ A :: Γ] |ₕ [y ∶ B :: Δ] ∧ Γ' ~ x ∶ C ⨂ D :: Γᵣ‚ Δᵣ := by
+      have hxRHS : (x ∶ C ⨂ D :: Γᵣ‚ Δᵣ) ∈
+        𝒢ᵣ |ₕ [x ∶ C ⨂ D :: Γᵣ‚ Δᵣ] |ₕ [y ∶ E ⅋ F :: Ξᵣ] := by simp
+      have ⟨Ξ, hΞ, hPΞ⟩ := HyperEnv.Perm_mem hP_pre hxRHS
+      simp only [HasPerm.perm] at hPΞ
+      simp only [List.append_assoc, List.cons_append, List.nil_append, List.mem_append,
+        List.mem_cons, List.not_mem_nil, or_false] at hΞ
+      rcases hΞ with h1 | h2 | h3
+      · exfalso
+        exact (HyperEnv.not_mem_names_iff.mp hx𝒢 Ξ _ h1)
+          ((List.Perm.mem_iff (a := x ∶ C ⨂ D) hPΞ.symm).mp (by simp))
+      · subst h2
+        have hxin := (List.Perm.mem_iff (a := x ∶ C ⨂ D) hPΞ).mpr (by simp)
+        simp only [List.mem_cons, Prod.mk.injEq, true_and] at hxin
+        rcases hxin with ⟨rfl, _⟩ | h
+        · refine ⟨(x ∶ C ⨂ D :: Γ), by simp, hPΞ⟩
+        · exfalso ; exact hxΓ (Env.mem_pair_fst_in_names _ h)
+      · subst h3
+        have hxin := (List.Perm.mem_iff (a := x ∶ C ⨂ D) hPΞ).mpr (by simp)
+        simp only [List.mem_cons, Prod.mk.injEq] at hxin
+        rcases hxin with ⟨rfl, _⟩ | h
+        · simp only [Env.disjoint, Env.names_distributes, Finset.singleton_union,
+          Finset.disjoint_insert_right, Finset.mem_insert, Env.mem_pair_fst_in_names_iff, true_or,
+          not_true_eq_false, Finset.disjoint_insert_left, not_exists, false_and] at hDΓΔ
+        · exfalso ; exact hxΔ (Env.mem_pair_fst_in_names _ h)
+    have hyLHS : ∃ Δ', Δ' ∈ 𝒢 |ₕ [x ∶ A :: Γ] |ₕ [y ∶ B :: Δ] ∧ Δ' ~ y ∶ E ⅋ F :: Ξᵣ := by
+      have hyRHS : (y ∶ E ⅋ F :: Ξᵣ) ∈ 𝒢ᵣ |ₕ [x ∶ C ⨂ D :: Γᵣ‚ Δᵣ] |ₕ [y ∶ E ⅋ F :: Ξᵣ] := by simp
+      have ⟨Ξ, hΞ, hPΞ⟩ := HyperEnv.Perm_mem hP_pre hyRHS
+      simp only [HasPerm.perm] at hPΞ
+      simp only [List.append_assoc, List.cons_append, List.nil_append, List.mem_append,
+        List.mem_cons, List.not_mem_nil, or_false] at hΞ
+      rcases hΞ with h1 | h2 | h3
+      · exfalso
+        exact (HyperEnv.not_mem_names_iff.mp hy𝒢 Ξ _ h1)
+          ((List.Perm.mem_iff (a := y ∶ E ⅋ F) hPΞ.symm).mp (by simp))
+      · subst h2
+        have hyin := (List.Perm.mem_iff (a := y ∶ E ⅋ F) hPΞ).mpr (by simp)
+        simp only [List.mem_cons, Prod.mk.injEq] at hyin
+        rcases hyin with ⟨rfl, _⟩ | h
+        · simp only [Env.disjoint, Env.names_distributes, Finset.singleton_union,
+          Finset.disjoint_insert_right, Finset.mem_insert, Env.mem_pair_fst_in_names_iff, true_or,
+          not_true_eq_false, Finset.disjoint_insert_left, not_exists, false_and] at hDΓΔ
+        · exfalso ; exact hyΓ (Env.mem_pair_fst_in_names _ h)
+      · subst h3
+        have hyin := (List.Perm.mem_iff (a := y ∶ E ⅋ F) hPΞ).mpr (by simp)
+        simp only [List.mem_cons, Prod.mk.injEq, true_and] at hyin
+        rcases hyin with ⟨rfl, _⟩ | h
+        · refine ⟨(y ∶ E ⅋ F :: Δ), by simp, hPΞ⟩
+        · exfalso ; exact hyΔ (Env.mem_pair_fst_in_names _ h)
+    simp only [List.append_assoc, List.cons_append, List.nil_append, List.mem_append, List.mem_cons,
+      List.not_mem_nil, or_false] at hxLHS hyLHS
+    rcases hxLHS with ⟨Γ', hΓ', hPΓ'⟩
+    rcases hyLHS with ⟨Δ', hΔ', hPΔ'⟩
+    rcases hΓ' with h1 | h2 | h3
+    · exfalso
+      exact HyperEnv.not_mem_names_iff.mp
+        hx𝒢 Γ' _ h1 ((List.Perm.mem_iff (a := x ∶ C ⨂ D) hPΓ'.symm).mp (by simp))
+    · subst h2
+      rcases hΔ' with h4 | h5 | h6
+      · exfalso
+        exact HyperEnv.not_mem_names_iff.mp
+          hy𝒢 Δ' _ h4 ((List.Perm.mem_iff (a := y ∶ E ⅋ F) hPΔ'.symm).mp (by simp))
+      · subst h5
+        have hyin := (List.Perm.mem_iff (a := y ∶ E ⅋ F) hPΔ').mpr (by simp)
+        simp only [List.mem_cons, Prod.mk.injEq] at hyin
+        rcases hyin with ⟨rfl, _⟩ | h
+        · simp only [Env.disjoint, Env.names_distributes, Finset.singleton_union,
+          Finset.disjoint_insert_right, Finset.mem_insert, Env.mem_pair_fst_in_names_iff, true_or,
+          not_true_eq_false, Finset.disjoint_insert_left, not_exists, false_and] at hDΓΔ
+        · exfalso ; exact hyΓ (Env.mem_pair_fst_in_names _ h)
+      · subst h6
+        have hx_eq := (List.Perm.mem_iff (a := x ∶ C ⨂ D) hPΓ').mpr (by simp)
+        simp only [List.mem_cons, Prod.mk.injEq, true_and] at hx_eq
+        rcases hx_eq with ⟨rfl, hA_eq⟩ | hx_eq
+        · have hy_eq := (List.Perm.mem_iff (a := y ∶ E ⅋ F) hPΔ').mpr (by simp)
+          simp only [List.mem_cons, Prod.mk.injEq, true_and] at hy_eq
+          rcases hy_eq with ⟨rfl, hB_eq⟩ | hy_eq
+          · have hPΓ := List.Perm.cons_inv hPΓ'
+            have hPΔ := List.Perm.cons_inv hPΔ'
+            refine ⟨C, D, E, F, Γᵣ, Δᵣ, rfl, rfl, hPΓ, ?_⟩
+            have hP1 : [x ∶ C ⨂ D :: Γ] ~ [x ∶ C ⨂ D :: Γᵣ‚ Δᵣ] :=
+              HyperEnv.Perm_singleton_singleton.mpr (List.Perm.cons _ hPΓ)
+            have hP2 : [y ∶ E ⅋ F :: Δ] ~ [y ∶ E ⅋ F :: Ξᵣ] :=
+              HyperEnv.Perm_singleton_singleton.mpr (List.Perm.cons _ hPΔ)
+            have hP3 : 𝒢ᵣ |ₕ [x ∶ C ⨂ D :: Γ] |ₕ [y ∶ E ⅋ F :: Δ] ~
+              𝒢ᵣ |ₕ [x ∶ C ⨂ D :: Γᵣ‚ Δᵣ] |ₕ [y ∶ E ⅋ F :: Ξᵣ] :=
+              HyperEnv.Perm.merge (HyperEnv.Perm.merge (HyperEnv.Perm.refl _) hP1) hP2
+            have hP4 := hP_pre.trans hP3.symm
+            apply HyperEnv.Perm_merge_cancel_right at hP4
+            apply HyperEnv.Perm_merge_cancel_right at hP4
+            have hP5 := hP_post.trans (HyperEnv.Perm.merge
+              (HyperEnv.Perm.merge (HyperEnv.Perm.merge hP4.symm
+                (HyperEnv.Perm.refl _)) (HyperEnv.Perm.refl _)) (HyperEnv.Perm.refl _))
+            have hP6 : [y' ∶ E :: y ∶ F :: Ξᵣ] ~ [y' ∶ E :: y ∶ F :: Δ] :=
+              HyperEnv.Perm_singleton_singleton.mpr (List.Perm.cons _ (List.Perm.cons _ hPΔ.symm))
+            exact hP5.trans (HyperEnv.Perm.merge (HyperEnv.Perm.refl _) hP6)
+          · exfalso ; exact hyΔ (Env.mem_pair_fst_in_names _ hy_eq)
+        · exfalso ; exact hxΓ (Env.mem_pair_fst_in_names _ hx_eq)
+    · subst h3
+      have hxin := (List.Perm.mem_iff (a := x ∶ C ⨂ D) hPΓ').mpr (by simp)
+      simp only [List.mem_cons] at hxin
+      rcases hxin with ⟨rfl, _⟩ | h
+      · simp only [Env.disjoint, Env.names_distributes, Finset.singleton_union,
+        Finset.disjoint_insert_right, Finset.mem_insert, Env.mem_pair_fst_in_names_iff, true_or,
+        not_true_eq_false, Finset.disjoint_insert_left, not_exists, false_and] at hDΓΔ
+      · exfalso ; exact hxΔ (Env.mem_pair_fst_in_names _ h)
+  · obtain ⟨𝒢ᵣ, Γᵣ, Δᵣ, Ξᵣ, C, D, E, F, hP_pre, _⟩ := h_right
+    have ⟨hdn, hpw⟩ := Typing_preserves_linearity 𝒟
+    have ⟨⟨hx𝒢, hxΓ, hxΔ⟩, ⟨hy𝒢, hyΓ, hyΔ⟩⟩ := Typing_res_fresh 𝒟
+    simp only [List.append_assoc, List.cons_append, List.nil_append,
+      HyperEnv.PairwiseDisjoint_merge, List.mem_cons, List.not_mem_nil, or_false, forall_eq_or_imp,
+      Env.names_distributes, Finset.singleton_union, Finset.disjoint_insert_right,
+      Env.mem_pair_fst_in_names_iff, not_exists, forall_eq] at hpw
+    have hDΓΔ := HyperEnv.PairwiseDisjoint_implies_disjoint hpw.2.1
+    have hxRHS : (x ∶ C ⨂ D :: Γᵣ ++ Δᵣ ++ y ∶ E ⅋ F :: Ξᵣ) ∈
+      𝒢ᵣ |ₕ [x ∶ C ⨂ D :: Γᵣ ++ Δᵣ ++ y ∶ E ⅋ F :: Ξᵣ] := by simp
+    have ⟨Γ', hΓ', hPΓ'⟩:= HyperEnv.Perm_mem hP_pre hxRHS
+    simp only [HasPerm.perm, List.cons_append, List.append_assoc] at hPΓ'
+    simp only [List.append_assoc, List.cons_append, List.nil_append, List.mem_append, List.mem_cons,
+      List.not_mem_nil, or_false] at hΓ'
+    rcases hΓ' with h1 | h2 | h3
+    · exfalso
+      exact HyperEnv.not_mem_names_iff.mp hx𝒢 Γ' _ h1
+        ((List.Perm.mem_iff (a := x ∶ C ⨂ D) hPΓ').mpr (by simp))
+    · subst h2
+      have hyin : (y, E ⅋ F) ∈ x ∶ C ⨂ D :: (Γᵣ ++ (Δᵣ ++ y ∶ E ⅋ F :: Ξᵣ)) := by simp
+      have hyinΓ' := (List.Perm.mem_iff hPΓ'.symm).mp hyin
+      simp only [List.mem_cons, Prod.mk.injEq] at hyinΓ'
+      rcases hyinΓ' with ⟨rfl, _⟩ | h
+      · simp only [Env.disjoint, Env.names_distributes, Finset.singleton_union,
+        Finset.disjoint_insert_right, Finset.mem_insert, Env.mem_pair_fst_in_names_iff, true_or,
+        not_true_eq_false, Finset.disjoint_insert_left, not_exists, false_and] at hDΓΔ
+      · exfalso ; exact hyΓ (Env.mem_pair_fst_in_names _ h)
+    · subst h3
+      have hxin : (x, C ⨂ D) ∈ x ∶ C ⨂ D :: (Γᵣ ++ (Δᵣ ++ y ∶ E ⅋ F :: Ξᵣ)) := by simp
+      have hxinΔ' := (List.Perm.mem_iff hPΓ').mpr hxin
+      simp only [List.mem_cons, Prod.mk.injEq] at hxinΔ'
+      rcases hxinΔ' with ⟨rfl, _⟩ | h
+      · simp only [Env.disjoint, Env.names_distributes, Finset.singleton_union,
+        Finset.disjoint_insert_right, Finset.mem_insert, Env.mem_pair_fst_in_names_iff, true_or,
+        not_true_eq_false, Finset.disjoint_insert_left, not_exists, false_and] at hDΓΔ
+      · exfalso ; exact hxΔ (Env.mem_pair_fst_in_names _ h)
