PiLL/Semantics/JudgementStep/MultiStep.lean
@@ -1,0 +1,15 @@
+import PiLL.Semantics.JudgementStep.Basic
+
+inductive MTSTₘ : {n n' : Nat} → {𝒢 𝒢' : HyperEnv} → {P P' : Proc} →
+  Typing n P 𝒢 → Lbls → Typing n' P' 𝒢' → Prop where
+  | refl {n : Nat} {P : Proc} {𝒢 : HyperEnv} {𝒟 : Typing n P 𝒢} :
+    MTSTₘ 𝒟 (ε) 𝒟
+  | stepR {n n' n'' : Nat} {l : Lbl} {ls : Lbls} {𝒢 𝒢' 𝒢'' : HyperEnv} {P P' P'' : Proc}
+    (𝒟  : Typing n P 𝒢) (𝒟' : Typing n' P' 𝒢') (𝒟'' : Typing n'' P'' 𝒢'') :
+    (MTSTₘ 𝒟 ls 𝒟'') → (𝒟'' -[l]-> 𝒟') →
+    -------------------------------------
+          MTSTₘ 𝒟 (ls ∷ₗ l) 𝒟'
+
+instance {n n' : Nat} {𝒢 𝒢' : HyperEnv} {P P' : Proc} :
+  HasMultiStep (Typing n P 𝒢) Lbls (Typing n' P' 𝒢') where
+  step 𝒟 l 𝒟' := MTSTₘ 𝒟 l 𝒟'
