PiLL/Semantics/JudgementStep/Properties/Linearity.lean
@@ -1,0 +1,34 @@
+import PiLL.Model.Judgement.Properties.Names
+import PiLL.Semantics.JudgementStep.Basic
+import PiLL.Semantics.JudgementStep.Properties.Names
+
+lemma TypingStepₘ_par_preserves_disjoint {n : Nat} {Q Q' R : Proc} {𝒥 𝒥' 𝒦 : HyperEnv} {l' : Lbl}
+  {hTQ : n ⊢ Q ∷ 𝒥} {hTQ' : n ⊢ Q' ∷ 𝒥'} (hTR : n ⊢ R ∷ 𝒦)
+  (hStep : TypingStepₘ hTQ l' hTQ') (hD : 𝒥.disjoint 𝒦) (disj : l'.i ∩ R.f = ∅) :
+  𝒥'.disjoint 𝒦 := by
+    have hsub := TypingStepₘ_names_bound hStep
+    simp only [HyperEnv.disjoint] at hsub hD
+    have hnf := Typing_f_eq_names hTR
+    have : Disjoint (𝒥.names ∪ l'.i) 𝒦.names := by
+      simp only [hnf, Finset.disjoint_union_left, hD, true_and] at disj ⊢
+      exact Finset.disjoint_iff_inter_eq_empty.mpr disj
+    exact Disjoint.mono_left hsub this
+
+lemma TypingStepₘ_syn_preserves_disjoint {n : Nat} {P P' Q Q' : Proc}
+  {𝒥 𝒥' 𝒦 𝒦' : HyperEnv} {l' l'' : Act} {hTP : n ⊢ P ∷ 𝒥} {hTP' : n ⊢ P' ∷ 𝒥'}
+  {hTQ : n ⊢ Q ∷ 𝒦} {hTQ' : n ⊢ Q' ∷ 𝒦'} (hStepPP' : TypingStepₘ hTP l' hTP')
+  (hStepQQ' : TypingStepₘ hTQ l'' hTQ') (hD : 𝒥.disjoint 𝒦)
+  (disj : (l' |ₗ l'').i ∩ (P |ₚ Q).f = ∅) (lwf : (l' |ₗ l'').WF) :
+  𝒥'.disjoint 𝒦' := by
+  have hsubRR' := TypingStepₘ_names_bound hStepPP'
+  have hsubQQ' := TypingStepₘ_names_bound hStepQQ'
+  have hlwf := Finset.disjoint_iff_inter_eq_empty.mpr lwf
+  have hdisj := Finset.disjoint_iff_inter_eq_empty.mpr disj
+  have hnfR := Typing_f_eq_names hTP
+  have hnfQ := Typing_f_eq_names hTQ
+  simp only [Proc.f_par, Lbl.i_par'] at hdisj
+  simp only [hnfR, hnfQ, Finset.disjoint_union_left, Finset.disjoint_union_right] at hdisj
+  rcases hdisj with ⟨⟨h1, h2⟩, ⟨h3, h4⟩⟩
+  apply Disjoint.mono hsubRR' hsubQQ'
+  simp only [Finset.disjoint_union_left, Finset.disjoint_union_right]
+  refine ⟨⟨hD, h3⟩, h2.symm, hlwf⟩
