PiLL/Semantics/JudgementStep/Properties/Names.lean
@@ -1,0 +1,94 @@
+import PiLL.Semantics.JudgementStep.Basic
+import PiLL.Model.HyperEnvironment.Lemmas.Basic
+
+lemma TypingStepₘ_names_bound {n n' : Nat} {P P' : Proc} {𝒢 𝒢' : HyperEnv} {l : Lbl}
+  {𝒟 : n ⊢ P ∷ 𝒢} {𝒟' : n' ⊢ P' ∷ 𝒢'}
+  (hStep : TypingStepₘ 𝒟 l 𝒟') :
+  𝒢'.names ⊆ 𝒢.names ∪ l.i := by
+  induction hStep
+  case one =>
+    simp only [List.empty_eq, HyperEnv.names_nil, HyperEnv.names_cons, Env.names_distributes,
+      Env.names_nil, Finset.union_empty, Lbl.i, iNamesAct, Finset.subset_singleton_iff,
+      Finset.empty_ne_singleton, or_false]
+  case bot =>
+    simp only [HyperEnv.names_cons, HyperEnv.names_nil, Finset.union_empty, Env.names_distributes,
+      Finset.singleton_union, Lbl.i, iNamesAct, Finset.subset_insert]
+  case tensor Γ Δ _ x y _ _ _ _ _ _ _ =>
+    simp only [HyperEnv.names_merge, HyperEnv.names_singleton,
+      Env.names_distributes, Lbl.i, iNamesAct, Env.names_merge]
+    rw [Finset.union_comm, Finset.union_assoc, Finset.union_comm _ Γ.names,
+      ← Finset.union_assoc Δ.names _, Finset.union_comm Δ.names Γ.names]
+    simp only [← Finset.union_assoc, subset_refl]
+  case parr =>
+    simp only [HyperEnv.names_singleton, Env.names_distributes, Lbl.i, iNamesAct]
+    rw [Finset.union_comm]
+  case tensor_parr | one_bot =>
+    simp only [HyperEnv.names_merge, HyperEnv.names_cons, Env.names_merge, HyperEnv.names_nil,
+      Finset.union_empty, List.append_assoc, Lbl.i, subset_refl]
+  case par₁ ih =>
+    simp only [HyperEnv.names_merge]
+    intro y hy
+    simp only [Finset.mem_union] at hy ⊢
+    rcases hy with hy𝒢' | hyℋ
+    · have := ih hy𝒢'
+      simp only [Finset.mem_union] at this
+      rcases this with h1 | h2
+      · simp only [h1, true_or, Lbl.i, iNamesAct]
+      · simp only [h2, or_true]
+    · simp only [hyℋ, or_true, Lbl.i, iNamesAct, true_or]
+  case par₂ ih =>
+    simp only [HyperEnv.names_merge]
+    intro y hy
+    simp only [Finset.mem_union] at hy ⊢
+    rcases hy with hy𝒢 | hyℋ'
+    · simp only [hy𝒢, true_or, Lbl.i, iNamesAct]
+    · have := ih hyℋ'
+      simp only [Finset.mem_union] at this
+      rcases this with h1 | h2
+      · simp only [h1, or_true, Lbl.i, iNamesAct, true_or]
+      · simp only [h2, or_true]
+  case syn ih1 ih2 =>
+    simp only [HyperEnv.names_merge]
+    intro y hy
+    simp only [Finset.mem_union] at hy ⊢
+    rcases hy with hy𝒢' | hyℋ'
+    · have := ih1 hy𝒢'
+      simp only [Finset.mem_union] at this
+      rcases this with h1 | h2
+      · simp only [h1, true_or, Lbl.i, iNamesAct, Finset.mem_union]
+      · simp only [Lbl.i_par', Finset.mem_union, h2, true_or, or_true]
+    · have := ih2 hyℋ'
+      simp only [Finset.mem_union] at this
+      rcases this with h1 | h2
+      · simp only [h1, or_true, Lbl.i, iNamesAct, Finset.mem_union, true_or]
+      · simp only [Lbl.i_par', Finset.mem_union, h2, or_true]
+  case res 𝒢' _ Γ' _ Δ' _ _ A _ _ _ _ _ huniq' x y hneq hx hy hx' hy' hlx hly hStep ih =>
+    intro a ha
+    simp only [HyperEnv.names_merge, HyperEnv.names_cons, Env.names_merge, HyperEnv.names_nil,
+      Finset.union_empty, Finset.mem_union, List.append_assoc, List.cons_append,
+      List.nil_append, Env.names_distributes, Finset.singleton_union, Finset.union_insert,
+      Finset.insert_union, Finset.union_assoc] at ha ih ⊢
+    have haLHS : a ∈ insert y (insert x (𝒢'.names ∪ (Γ'.names ∪ Δ'.names))) := by
+      simp only [Finset.mem_insert, Finset.mem_union, ha, or_true]
+    have haRHS := ih haLHS
+    simp only [Finset.mem_insert, Finset.mem_union] at haRHS
+    simp only [Finset.notMem_union, and_assoc] at hx hy hx' hy'
+    obtain ⟨hxPf', hx𝒢', hxΓ', hxΔ'⟩ := hx'
+    obtain ⟨hyPf', hy𝒢', hyΓ', hyΔ'⟩ := hy'
+    rcases haRHS with rfl | rfl | h
+    · rcases ha with h1 | h2 | h3
+      · exfalso ; apply hy𝒢' h1
+      · exfalso ; apply hyΓ' h2
+      · exfalso ; apply hyΔ' h3
+    · rcases ha with h1 | h2 | h3
+      · exfalso ; apply hx𝒢' h1
+      · exfalso ; apply hxΓ' h2
+      · exfalso ; apply hxΔ' h3
+    · exact h
+  case perm_hyper hP hP' _ ih =>
+    rw [← (HyperEnv.names_eq_of_perm hP), ← (HyperEnv.names_eq_of_perm hP')]
+    exact ih
+  case perm_env hP _ ih =>
+    simp only [HyperEnv.names_cons, Finset.union_assoc] at ⊢ ih
+    rw [← (Env.names_eq_of_perm hP)]
+    exact ih
