PiLL/Semantics/JudgementStep/Properties/WellFormed.lean
@@ -1,0 +1,7 @@
+import PiLL.Semantics.JudgementStep.Basic
+
+theorem TypingStepₘ.preserves_WF {n n' 𝒢 𝒢' P P'}
+  (𝒟 : n ⊢ P ∷ 𝒢) (𝒟' : n' ⊢ P' ∷ 𝒢') (l : Lbl) :
+  TypingStepₘ 𝒟 l 𝒟' → l.WF := by
+  intro h
+  induction h <;> simp_all only [Lbl.WF]
