PiLL/SessionFidelity/Typability.lean
@@ -1,0 +1,305 @@
+import PiLL.Model.Judgement.Inversion.Lemmas
+import PiLL.Semantics.JudgementStep.Inversion.One_Bot
+import PiLL.Semantics.JudgementStep.Inversion.Res
+import PiLL.Semantics.JudgementStep.Inversion.Tensor_parr
+import PiLL.Semantics.JudgementStep.Properties.Linearity
+import PiLL.Semantics.ProcStep.Basic
+
+theorem typability_subject_reductionₘ
+  {n : Nat} {𝒢 : HyperEnv} {P P' : Proc} {l : Lbl}
+  (𝒟 : Typing n P 𝒢) (hPS : ProcStepₘ P l P') :
+  ∃ (𝒢' : HyperEnv) (𝒟' : Typing n P' 𝒢'),
+    TypingStepₘ 𝒟 l 𝒟' := by
+  induction hPS generalizing n 𝒢
+  case one =>
+    obtain ⟨hP, 𝒟'⟩ := Typing_inv_one 𝒟
+    have ⟨Δ, heq, hPΔ⟩:= HyperEnv.Perm_singleton_inv hP.symm
+    simp only [HasPerm.perm, List.singleton_perm] at hPΔ
+    subst hPΔ heq
+    use ∅, 𝒟'
+    apply TypingStepₘ.one
+  case bot =>
+    obtain ⟨Γ, hP, 𝒟'⟩ := Typing_inv_bot 𝒟
+    have := HyperEnv.Nodup_perm hP (Typing_preserves_linearity 𝒟).1
+    simp only [HyperEnv.Nodup_singleton, Env.Nodup_cons] at this
+    obtain ⟨hxΓ, _⟩ := this
+    use [Γ], 𝒟'
+    exact TypingStepₘ.perm_hyper (𝒟' := 𝒟') hP.symm (by rfl) (TypingStepₘ.bot (hF := hxΓ))
+  case tensor Q x y hF =>
+    obtain ⟨A, B, Γ, Δ, L, hP, 𝒟'⟩ := Typing_inv_tensor 𝒟
+    simp only [Finset.singleton_union, Finset.mem_insert, not_or, ← ne_eq] at hF
+    obtain ⟨hF1, hF2⟩ := hF
+    obtain ⟨z, hz⟩ := exists_one_fresh (L ∪ {y} ∪ Q.f)
+    simp only [Finset.union_singleton, Finset.insert_union, Finset.mem_insert, Finset.mem_union,
+      not_or, ← ne_eq] at hz
+    obtain ⟨hzy, hz, hfz⟩ := hz
+    have 𝒟z := (𝒟' z hz)
+    have hfy := Proc.not_mem_f_open hzy hfz hF2
+    rw [(Typing_f_eq_names 𝒟z)] at hfy
+    have ⟨hyΓ, hyΔ⟩ : y ∉ Γ.names ∧ y ∉ Δ.names := by
+      constructor <;> (intro hc ; simp [hc] at hfy)
+    have hy : y ∉ {x} ∪ Q.f ∪ Γ.names ∪ Δ.names := by simp [hF2, hyΓ, hyΔ, hF1]
+    have ⟨hnd, hpw⟩ := Typing_preserves_linearity 𝒟
+    have hnd' := HyperEnv.Nodup_perm hP hnd
+    simp only [HyperEnv.Nodup_singleton, Env.Nodup_cons, Env.names_merge,
+      Finset.mem_union, not_or] at hnd'
+    have 𝒟y := Typing_tensor_all_fresh 𝒟' y hy
+    · use [y ∶ A :: Γ] |ₕ [x ∶ B :: Δ], 𝒟y
+      apply TypingStepₘ.perm_hyper hP.symm (by rfl)
+      apply TypingStepₘ.tensor
+      · exact hnd'.1
+      · exact 𝒟'
+      · exact hy
+  case parr Q x y hF =>
+    obtain ⟨A, B, Γ, L, hP, 𝒟'⟩ := Typing_inv_parr 𝒟
+    simp only [Finset.singleton_union, Finset.mem_insert, not_or, ← ne_eq] at hF
+    obtain ⟨hF1, hF2⟩ := hF
+    obtain ⟨z, hz⟩ := exists_one_fresh (L ∪ {y} ∪ Q.f)
+    simp only [Finset.union_singleton, Finset.insert_union, Finset.mem_insert, Finset.mem_union,
+      not_or, ← ne_eq] at hz
+    obtain ⟨hzy, hz, hfz⟩ := hz
+    have 𝒟z := (𝒟' z hz)
+    have hfy := Proc.not_mem_f_open hzy hfz hF2
+    rw [(Typing_f_eq_names 𝒟z)] at hfy
+    have hyΓ : y ∉ Γ.names := by intro hc ; simp [hc] at hfy
+    have hy : y ∉ {x} ∪ Q.f ∪ Γ.names := by simp [hF2, hyΓ, hF1]
+    have ⟨hnd, hpw⟩ := Typing_preserves_linearity 𝒟
+    have hnd' := HyperEnv.Nodup_perm hP hnd
+    simp only [HyperEnv.Nodup_singleton, Env.Nodup_cons] at hnd'
+    have 𝒟y := Typing_parr_all_fresh 𝒟' y hy
+    · use [y ∶ A :: x ∶ B :: Γ], 𝒟y
+      apply TypingStepₘ.perm_hyper hP.symm (by rfl)
+      apply TypingStepₘ.parr
+      · exact hnd'.1
+      · exact 𝒟'
+      · exact hy
+  case par₁ disj ih =>
+    have ⟨𝒥, 𝒦, hP, hTQ, hTR, hD⟩ := Typing_inv_par 𝒟
+    have ⟨𝒥', hTQ', hStepQQ'⟩ := ih hTQ
+    have hD' : Disjoint 𝒥'.names 𝒦.names :=
+      TypingStepₘ_par_preserves_disjoint hTR hStepQQ' hD disj
+    use 𝒥' |ₕ 𝒦, (Typing.mix hD' hTQ' hTR)
+    apply TypingStepₘ.perm_hyper hP.symm (by rfl)
+    · apply TypingStepₘ.par₁ hStepQQ' disj
+      · exact hD
+      · exact hD'
+      · exact hTR
+  case par₂ disj ih =>
+    have ⟨𝒦, 𝒥, hP, hTR, hTQ, hD⟩ := Typing_inv_par 𝒟
+    have ⟨𝒥', hTQ', hStepQQ'⟩ := ih hTQ
+    have hD' : Disjoint 𝒦.names 𝒥'.names :=
+      (TypingStepₘ_par_preserves_disjoint hTR hStepQQ' hD.symm disj).symm
+    use 𝒦 |ₕ 𝒥', (Typing.mix hD' hTR hTQ')
+    apply TypingStepₘ.perm_hyper hP.symm (by rfl)
+    · apply TypingStepₘ.par₂ hStepQQ' disj
+      · exact hD
+      · exact hD'
+      · exact hTR
+  case syn l' l'' _ _ disj lwf ih1 ih2 =>
+    have ⟨𝒥, 𝒦, hP, hTR, hTQ, hD⟩ := Typing_inv_par 𝒟
+    have ⟨𝒥', hTR', hStepRR'⟩ := ih1 hTR
+    have ⟨𝒦', hTQ', hStepQQ'⟩ := ih2 hTQ
+    have hD' : 𝒥'.disjoint 𝒦' :=
+      TypingStepₘ_syn_preserves_disjoint hStepRR' hStepQQ' hD disj lwf
+    use 𝒥' |ₕ 𝒦', (Typing.mix ?_ hTR' hTQ')
+    · apply TypingStepₘ.perm_hyper hP.symm (by rfl)
+      · apply TypingStepₘ.syn
+        · exact hD
+        · exact hD'
+        · exact hStepRR'
+        · exact hStepQQ'
+        · exact disj
+        · exact lwf
+    · exact hD'
+  case one_bot Q Q' x y hxQf hyQf hxy hPS ih =>
+    have ⟨A, Γ, Δ, ℋ, L, hP, 𝒟'⟩ := Typing_inv_res 𝒟
+    have hNames := Typing_f_eq_names 𝒟
+    simp only [Proc.f_cut, HyperEnv.names_eq_of_perm hP, HyperEnv.names_merge, HyperEnv.names_cons,
+      Env.names_merge, HyperEnv.names_nil, Finset.union_empty] at hNames
+    let hxQf' := hxQf
+    let hyQf' := hyQf
+    simp only [hNames, Finset.mem_union, not_or] at hxQf' hyQf'
+    obtain ⟨hxℋ, hxΓ, hxΔ⟩ := hxQf'
+    obtain ⟨hyℋ, hyΓ, hyΔ⟩ := hyQf'
+    have hx_bound_t : x ∉ Q.f ∪ ℋ.names ∪ Γ.names ∪ Δ.names := by
+      simp only [Finset.mem_union, not_or]
+      exact ⟨⟨⟨hxQf, hxℋ⟩, hxΓ⟩, hxΔ⟩
+    have hy_bound_t : y ∉ (Q.f ∪ ℋ.names ∪ Γ.names ∪ Δ.names) := by
+      simp only [Finset.mem_union, not_or]
+      exact ⟨⟨⟨hyQf, hyℋ⟩, hyΓ⟩, hyΔ⟩
+    have hx_bound : x ∉ ({y} ∪ Q.f ∪ ℋ.names ∪ Δ.names) := by
+      simp only [Finset.mem_union, Finset.mem_singleton, not_or, ← ne_eq]
+      exact ⟨⟨⟨hxy, hxQf⟩, hxℋ⟩, hxΔ⟩
+    have hy_bound : y ∉ (Q.f ∪ ℋ.names ∪ Δ.names) := by
+      simp only [Finset.mem_union, not_or]
+      exact ⟨⟨hyQf, hyℋ⟩, hyΔ⟩
+    have 𝒟xy := (Typing_res_all_fresh 𝒟' x y hx_bound_t hy_bound_t hxy)
+    have ⟨_, _, hTS_t⟩ := ih 𝒟xy
+    have ⟨hA, hB, hΓ, _⟩ := TypingStepₘ_inv_one_bot_source 𝒟xy hTS_t
+    subst hA hΓ
+    rw! [hB] at *
+    have := (Typing_one_bot_all_fresh 𝒟' x y hx_bound hy_bound)
+    obtain ⟨𝒢', 𝒟'', hTS'⟩ := ih (Typing_one_bot_all_fresh 𝒟' x y hx_bound hy_bound)
+    have ⟨_, _, _, hP𝒢'⟩ := TypingStepₘ_inv_one_bot_source this hTS'
+    refine ⟨𝒢', 𝒟'', ?_⟩
+    apply TypingStepₘ.perm_hyper hP.symm hP𝒢'.symm
+    · apply TypingStepₘ.one_bot (𝒢' := 𝒢') (huniq := 𝒟') (hx := hx_bound) (hy := hy_bound)
+      · exact TypingStepₘ.perm_hyper (by rfl) hP𝒢' hTS'
+  case tensor_parr Q Q' x x' y y' hxQf hyQf hx'Qf hy'Qf hxQ'f hyQ'f hx'Q'f hy'Q'f
+    hxx' hxy hxy' hyx' hyy' hx'y' hPS ih =>
+    generalize heq : (𝑣⸨$N,$N⸩ Q) = R at 𝒟
+    induction 𝒟 generalizing Q <;> try contradiction
+    case exchange_env hP ih' =>
+      obtain ⟨𝒢_post, 𝒟_post, hTS_post⟩ := ih' hxQf hyQf hx'Qf hy'Qf hPS ih heq
+      expose_names
+      refine ⟨𝒢_post, 𝒟_post, ?_⟩
+      apply TypingStepₘ.perm_env hP hTS_post
+    case exchange_hyper hP ih' =>
+      obtain ⟨𝒢_post, 𝒟_post, hTS_post⟩ := ih' hxQf hyQf hx'Qf hy'Qf hPS ih heq
+      expose_names
+      refine ⟨𝒢_post, 𝒟_post, ?_⟩
+      apply TypingStepₘ.perm_hyper hP (by rfl) hTS_post
+    case cut 𝒢 Γ Δ _ A m L 𝒟 ih' =>
+      injection heq with hPQ
+      subst hPQ
+      have hNames := Typing_f_eq_names (Typing.cut L 𝒟)
+      simp only [Proc.f_cut, HyperEnv.names_merge, HyperEnv.names_cons, Env.names_merge,
+        HyperEnv.names_nil, Finset.union_empty] at hNames
+      let hxQf_t := hxQf
+      let hyQf_t := hyQf
+      let hxQf_t' := hx'Qf
+      let hyQf_t' := hy'Qf
+      simp only [hNames, Finset.mem_union, not_or] at hxQf_t hyQf_t hxQf_t' hyQf_t'
+      have hx_bound : x ∉ Q.f ∪ 𝒢.names ∪ Γ.names ∪ Δ.names := by
+        simp only [Finset.mem_union, not_or, and_assoc]
+        exact ⟨hxQf, hxQf_t⟩
+      have hy_bound : y ∉ Q.f ∪ 𝒢.names ∪ Γ.names ∪ Δ.names := by
+        simp only [Finset.mem_union, not_or, and_assoc]
+        exact ⟨hyQf, hyQf_t⟩
+      have hx'_bound : x' ∉ {y'} ∪ Q.f ∪ 𝒢.names ∪ Γ.names ∪ Δ.names := by
+        simp only [Finset.mem_union, Finset.mem_singleton, not_or, ← ne_eq, and_assoc]
+        exact ⟨hx'y', ⟨hx'Qf, hxQf_t'⟩⟩
+      have hy'_bound : y' ∉ Q.f ∪ 𝒢.names ∪ Γ.names ∪ Δ.names := by
+        simp only [Finset.mem_union, not_or, and_assoc]
+        exact ⟨hy'Qf, hyQf_t'⟩
+      have 𝒟xy := Typing_res_all_fresh 𝒟 x y hx_bound hy_bound hxy
+      obtain ⟨𝒢_post, 𝒟_post, hTS_post⟩ := ih 𝒟xy
+      have ⟨C, D, E, F, Γ₁, Γ₂, hA, hA', hΓ, hP_post'⟩ :=
+        TypingStepₘ_inv_tensor_parr_source 𝒟xy hTS_post
+      subst hA
+      let hA'_t := hA'
+      simp only [Types.dual, Types.parr.injEq] at hA'_t
+      obtain ⟨hA'_t1, hA'_t2⟩ := hA'_t
+      subst hA'_t1 hA'_t2
+      have 𝒟xy_rw : m ⊢ Q⸨#x, #y⸩ ∷ 𝒢 |ₕ [x ∶ C ⨂ D :: Γ] |ₕ [y ∶ Cᗮ ⅋ Dᗮ :: Δ] := by
+        exact 𝒟xy
+      have hP_pre_rw : ∀ z w,
+        𝒢 |ₕ [z ∶ C ⨂ D :: Γ] |ₕ [w ∶ Cᗮ ⅋ Dᗮ :: Δ] ~
+        𝒢 |ₕ [z ∶ C ⨂ D :: Γ₁‚ Γ₂] |ₕ [w ∶ Cᗮ ⅋ Dᗮ :: Δ] := by
+        intros z w
+        exact HyperEnv.Perm_merge_cancel_right_inv (HyperEnv.Perm.merge (by rfl)
+          (HyperEnv.Perm_singleton_singleton.mpr (List.Perm.cons _ hΓ)))
+      have step_rw : TypingStepₘ 𝒟xy_rw (x⟦x'⟧ |ₗ y⸨y'⸩) 𝒟_post := by
+        apply TypingStepₘ.perm_hyper ?_ (by rfl) hTS_post
+        rw [hA']
+      have hTS_post' := TypingStepₘ.perm_hyper (hP_pre_rw x y) hP_post' step_rw
+      have 𝒟_post' := Typing.exchange_hyper 𝒟_post hP_post'
+      let L' := Q.f ∪ 𝒢.names ∪ (Γ₁‚ Γ₂).names ∪ Δ.names
+      have huinq_pre : ∀ x ∉ L', ∀ y ∉ L', x ≠ y →
+        m ⊢ Q⸨#x, #y⸩ ∷ 𝒢 |ₕ [x ∶ C ⨂ D :: Γ₁‚ Γ₂] |ₕ [y ∶ Cᗮ ⅋ Dᗮ :: Δ] := by
+        intros a ha b hb hab
+        have hΓ_names : Γ.names = (Γ₁‚ Γ₂).names := Env.names_eq_of_perm hΓ
+        have ha_bound : a ∉ Q.f ∪ 𝒢.names ∪ Γ.names ∪ Δ.names := by
+          simp only [L', hΓ_names, Finset.mem_union, not_or] at ⊢ ha
+          exact ha
+        have hb_bound : b ∉ Q.f ∪ 𝒢.names ∪ Γ.names ∪ Δ.names := by
+          simp only [L', hΓ_names, Finset.mem_union, not_or] at ⊢ hb
+          exact hb
+        have 𝒟ab := Typing_res_all_fresh 𝒟 a b ha_bound hb_bound hab
+        have 𝒟ab_rw : m ⊢ Q⸨#a, #b⸩ ∷ 𝒢 |ₕ [a ∶ C ⨂ D :: Γ] |ₕ [b ∶ Cᗮ ⅋ Dᗮ :: Δ] := by
+          exact 𝒟ab
+        exact Typing.exchange_hyper 𝒟ab (hP_pre_rw a b)
+      have hL' : x ∉ L' ∧ y ∉ L' ∧ x' ∉ L' ∧ y' ∉ L' := by
+        have hΓ_names : Γ.names = (Γ₁‚ Γ₂).names := Env.names_eq_of_perm hΓ
+        simp only [L', ← hΓ_names, Finset.mem_union, not_or]
+          at ⊢ hx_bound hy_bound hx'_bound hy'_bound
+        exact ⟨⟨⟨⟨hxQf, hx_bound.1.1.2⟩, hx_bound.1.2⟩, hx_bound.2⟩,
+               ⟨⟨⟨hyQf, hy_bound.1.1.2⟩, hy_bound.1.2⟩, hy_bound.2⟩,
+               ⟨⟨⟨hx'Qf, hx'_bound.1.1.2⟩, hx'_bound.1.2⟩, hx'_bound.2⟩,
+               ⟨⟨⟨hy'Qf, hy'_bound.1.1.2⟩, hy'_bound.1.2⟩, hy'_bound.2⟩⟩
+      have huniq_post : ∀ z ∉ L', ∀ w ∉ L', z ≠ w → ∀ z' ∉ L',
+        ∀ w' ∉ L', z' ≠ w' → z ≠ z' → z ≠ w' → w ≠ z' → w ≠ w' →
+        m ⊢ Q'⸨2 | #z, #w⸩⸨#z', #w'⸩ ∷
+          𝒢 |ₕ [z ∶ D :: Γ₂] |ₕ [z' ∶ C :: Γ₁] |ₕ [w' ∶ Cᗮ :: w ∶ Dᗮ :: Δ] := by
+        intros z hzL w hwL hzw z' hz'L w' hw'L hz'w' hzz' hzw' hwz' hww'
+        have hsubL' : 𝒢.names ∪ (Γ₂‚ Γ₁).names ∪ Δ.names ⊆ L' := by
+          simp only [Env.names_merge, Finset.union_assoc, L']
+          rw [← Finset.union_assoc Γ₂.names Γ₁.names _, Finset.union_comm _ Γ₁.names,
+            Finset.union_assoc]
+          exact Finset.subset_union_right
+        exact Typing_tensor_parr_post_all_fresh L' 𝒟_post' hL'.1 hL'.2.1 hL'.2.2.1 hL'.2.2.2
+          hsubL' hxQ'f hyQ'f hx'Q'f hy'Q'f hxx' hxy hxy' hyx' hyy' hx'y' z hzL w hwL
+          hzw z' hz'L w' hw'L hz'w' hzz' hzw' hwz' hww'
+      have hP_rw : 𝒢 |ₕ [(Γ₁‚ Γ₂)‚ Δ] ~  𝒢 |ₕ [Γ‚ Δ] := by
+        apply HyperEnv.Perm.merge (by rfl)
+        rw [HyperEnv.Perm_singleton_singleton]
+        apply List.Perm.append hΓ.symm (by rfl)
+      have hTS_raw := TypingStepₘ.tensor_parr
+        (L := L') (huniq := huinq_pre) (huniq' := huniq_post)
+        (hx := hL'.1) (hy := hL'.2.1) (hneq := hxy)
+        (hx' := hL'.2.2.1) (hy' := hL'.2.2.2) (hneq' := hx'y')
+        (hxx' := hxx') (hxy' := hxy') (hyx' := hyx') (hyy' := hyy')
+        (hxP := hxQf) (hyP := hyQf) (hx'P := hx'Qf) (hy'P := hy'Qf)
+        (hxP' := hxQ'f) (hyP' := hyQ'f) (hx'P' := hx'Q'f) (hy'P' := hy'Q'f)
+        hTS_post'
+      have hTS_final := TypingStepₘ.perm_hyper hP_rw HyperEnv.Perm_refl hTS_raw
+      exact ⟨_, _, hTS_final⟩
+  case res Q Q' l' x y hxy hFx hFy hlx hly hES ih =>
+    have ⟨A, Γ, Δ, ℋ, L, hP, 𝒟'⟩ := Typing_inv_res 𝒟
+    have hNames := Typing_f_eq_names 𝒟
+    simp only [Proc.f_cut, HyperEnv.names_eq_of_perm hP, HyperEnv.names_merge, HyperEnv.names_cons,
+      Env.names_merge, HyperEnv.names_nil, Finset.union_empty] at hNames
+    let hFx' := hFx
+    let hFy' := hFy
+    let hlx' := hlx
+    let hly' := hly
+    rw [hNames] at hFx' hFy'
+    simp only [Finset.mem_union, not_or, Finset.union_assoc] at hFx hFy hFx' hFy' hlx' hly'
+    obtain ⟨hlxf, hlxi⟩ := hlx'
+    obtain ⟨hlyf, hlyi⟩ := hly'
+    obtain ⟨hxℋ, hxΓ, hxΔ, hxQ'f⟩ := hFx'
+    obtain ⟨hyℋ, hyΓ, hyΔ, hyQ'f⟩ := hFy'
+    have hx_bound : x ∉ (Q.f ∪ ℋ.names ∪ Γ.names ∪ Δ.names) := by
+      simp only [Finset.mem_union, not_or]
+      exact ⟨⟨⟨hFx.1, hxℋ⟩, hxΓ⟩, hxΔ⟩
+    have hy_bound : y ∉ (Q.f ∪ ℋ.names ∪ Γ.names ∪ Δ.names) := by
+      simp only [Finset.mem_union, not_or]
+      exact ⟨⟨⟨hFy.1, hyℋ⟩, hyΓ⟩, hyΔ⟩
+    have 𝒟xy := (Typing_res_all_fresh 𝒟' x y hx_bound hy_bound hxy)
+    have ⟨𝒢xy', 𝒟xy', hTS_xy⟩ := ih 𝒟xy
+    -- FIXME: TypingStepₘ_inv_res_source has changed
+
+    have ⟨𝒢', Γ', Δ', hP'⟩ := TypingStepₘ_inv_res_source 𝒟xy hTS_xy hlx hly
+    have 𝒟xy' : n ⊢ Q'⸨#x, #y⸩ ∷ 𝒢' |ₕ [x ∶ A :: Γ'] |ₕ [y ∶ Aᗮ :: Δ'] :=
+      Typing.exchange_hyper 𝒟xy' hP'
+    let L' := Q'.f ∪ 𝒢'.names ∪ Γ'.names ∪ Δ'.names
+    have ⟨⟨hx𝒢', hxΓ', hxΔ'⟩, ⟨hy𝒢', hyΓ', hyΔ'⟩⟩ := Typing_res_fresh 𝒟xy'
+    have hxL' : x ∉ L' := by simp [L', hxQ'f, hx𝒢', hxΓ', hxΔ']
+    have hyL' : y ∉ L' := by simp [L', hyQ'f, hy𝒢', hyΓ', hyΔ']
+    have hEnv : 𝒢'.names ∪ Γ'.names ∪ Δ'.names ⊆ L' := by
+      intro a ha
+      simp only [L', Finset.mem_union] at ⊢ ha
+      rcases ha with h1 | hΔ'
+      · rcases h1 with h𝒢' | hΓ'
+        · left ; left ; right ; exact h𝒢'
+        · left ; right ; exact hΓ'
+      · right ; exact hΔ'
+    have 𝒟'_post_L' : ∀ z ∉ L', ∀ w ∉ L', z ≠ w →
+      n ⊢ Q'⸨#z, #w⸩ ∷ 𝒢' |ₕ [z ∶ A :: Γ'] |ₕ [w ∶ Aᗮ :: Δ'] := by
+      apply Typing_res_post_all_fresh L' 𝒟xy' hxL' hyL' hxQ'f hyQ'f hEnv hxy
+    have hTS_xy' : TypingStepₘ 𝒟xy l' 𝒟xy' :=
+      TypingStepₘ.perm_hyper (by rfl) hP' hTS_xy
+    refine ⟨𝒢' |ₕ [Γ'‚ Δ'], Typing.cut L' 𝒟'_post_L', ?_⟩
+    apply TypingStepₘ.perm_hyper hP.symm HyperEnv.Perm_refl
+    exact TypingStepₘ.res (L := L) (L' := L') (huniq := 𝒟') (huniq' := 𝒟'_post_L')
+      hxy hx_bound hy_bound hxL' hyL' hlx hly hTS_xy'
